main/hl/student/lean/HL/Hoare2.lean
@@ -925,7 +925,7 @@ theorem verification_conditions_correct (dec : Decorated)
 --  big and contain many conjuncts that are essentially trivial.
 
 example : decWhile.VerificationConditions := by
-  rw [Decorated.VerificationConditions, decWhile]
+  unfold Decorated.VerificationConditions decWhile
   simp only [DCom.VerificationConditions,
     DCom.postcondition]
   sorry
@@ -1934,14 +1934,13 @@ theorem hoare_asgn_weakest
 --  Show that your `havoc_pre` function from the `himp_hoare` exercise in
 --  the Hoare chapter returns a weakest precondition.
 
-namespace HimpHoare2
-open HimpHoare
+namespace Himp2
 
 theorem hoare_havoc_weakest (P Q : Assertion) (x : Ident)
-    (h : ValidHoareTriple P (Com.havoc x) Q) :
-    P ->> havoc_pre x Q := by
+    (h : Himp.ValidHoareTriple P (Himp.Com.havoc x) Q) :
+    P ->> Himp.havoc_pre x Q := by
   sorry
 
-end HimpHoare2
+end Himp2
 
--- Built on 2026-09-15 21:41 UTC
+-- Built on 2026-09-10 14:28 UTC
